mul_1 test and benchmark

code/mpfr/injected/add1sp_extracted.c
@@ -1,0 +1,1155 @@
+/* mpfr_add1sp -- internal function to perform a "real" addition
+   All the op must have the same precision
+
+Copyright 2004-2018 Free Software Foundation, Inc.
+Contributed by the AriC and Caramba projects, INRIA.
+
+This file is part of the GNU MPFR Library.
+
+The GNU MPFR Library is free software; you can redistribute it and/or modify
+it under the terms of the GNU Lesser General Public License as published by
+the Free Software Foundation; either version 3 of the License, or (at your
+option) any later version.
+
+The GNU MPFR Library is distributed in the hope that it will be useful, but
+WITHOUT ANY WARRANTY; without even the implied warranty of MERCHANTABILITY
+or FITNESS FOR A PARTICULAR PURPOSE.  See the GNU Lesser General Public
+License for more details.
+
+You should have received a copy of the GNU Lesser General Public License
+along with the GNU MPFR Library; see the file COPYING.LESSER.  If not, see
+http://www.gnu.org/licenses/ or write to the Free Software Foundation, Inc.,
+51 Franklin St, Fifth Floor, Boston, MA 02110-1301, USA. */
+
+#define MPFR_NEED_LONGLONG_H
+#include "mpfr-impl.h"
+
+#if MPFR_WANT_ASSERT >= 2
+/* Check the result of mpfr_add1sp with mpfr_add1.
+
+   Note: mpfr_add1sp itself has two algorithms: one always valid and one
+   faster for small precisions (up to 3 limbs). The latter one is disabled
+   if MPFR_GENERIC_ABI is defined. When MPFR_WANT_ASSERT >= 2, it could be
+   interesting to compare the results of these different algorithms. For
+   the time being, this is currently done by running the same code on the
+   same data with and without MPFR_GENERIC_ABI defined, where we have the
+   following comparisons in small precisions:
+     mpfr_add1sp slow <-> mpfr_add1 when MPFR_GENERIC_ABI is defined;
+     mpfr_add1sp fast <-> mpfr_add1 when MPFR_GENERIC_ABI is not defined.
+   By transitivity, the absence of failures implies that the 3 results are
+   the same.
+*/
+
+int mpfr_add1sp_ref (mpfr_ptr, mpfr_srcptr, mpfr_srcptr, mpfr_rnd_t);
+int mpfr_add1sp (mpfr_ptr a, mpfr_srcptr b, mpfr_srcptr c, mpfr_rnd_t rnd_mode)
+{
+  mpfr_t tmpa, tmpb, tmpc, tmpd;
+  mpfr_flags_t old_flags, flags, flags2;
+  int inexb, inexc, inexact, inexact2;
+
+  if (rnd_mode == MPFR_RNDF)
+    return mpfr_add1sp_ref (a, b, c, rnd_mode);
+
+  old_flags = __gmpfr_flags;
+
+  mpfr_init2 (tmpa, MPFR_PREC (a));
+  mpfr_init2 (tmpb, MPFR_PREC (b));
+  mpfr_init2 (tmpc, MPFR_PREC (c));
+
+  inexb = mpfr_set (tmpb, b, MPFR_RNDN);
+  MPFR_ASSERTN (inexb == 0);
+
+  inexc = mpfr_set (tmpc, c, MPFR_RNDN);
+  MPFR_ASSERTN (inexc == 0);
+
+  MPFR_ASSERTN (__gmpfr_flags == old_flags);
+
+  if (MPFR_GET_EXP (tmpb) < MPFR_GET_EXP (tmpc))
+    {
+      /* The sign for the result will be taken from the second argument
+         (= first input value, which is tmpb). */
+      MPFR_ALIAS (tmpd, tmpc, MPFR_SIGN (tmpb), MPFR_EXP (tmpc));
+      inexact2 = mpfr_add1 (tmpa, tmpd, tmpb, rnd_mode);
+    }
+  else
+    {
+      inexact2 = mpfr_add1 (tmpa, tmpb, tmpc, rnd_mode);
+    }
+  flags2 = __gmpfr_flags;
+
+  __gmpfr_flags = old_flags;
+  inexact = mpfr_add1sp_ref (a, b, c, rnd_mode);
+  flags = __gmpfr_flags;
+
+  if (! mpfr_equal_p (tmpa, a) || inexact != inexact2 /*|| flags != flags2*/)
+    {
+      fprintf (stderr, "add1 & add1sp return different values for %s\n"
+               "Prec_a = %lu, Prec_b = %lu, Prec_c = %lu\nB = ",
+               mpfr_print_rnd_mode (rnd_mode),
+               (unsigned long) MPFR_PREC (a),
+               (unsigned long) MPFR_PREC (b),
+               (unsigned long) MPFR_PREC (c));
+      mpfr_fdump (stderr, tmpb);
+      fprintf (stderr, "C = ");
+      mpfr_fdump (stderr, tmpc);
+      fprintf (stderr, "\nadd1  : ");
+      mpfr_fdump (stderr, tmpa);
+      fprintf (stderr, "add1sp: ");
+      mpfr_fdump (stderr, a);
+      fprintf (stderr, "Inexact sp = %d | Inexact = %d\n"
+               "Flags sp = %u | Flags = %u\n",
+               inexact, inexact2, flags, flags2);
+      MPFR_ASSERTN (0);
+    }
+  mpfr_clears (tmpa, tmpb, tmpc, (mpfr_ptr) 0);
+  return inexact;
+}
+# define mpfr_add1sp mpfr_add1sp_ref
+#endif  /* MPFR_WANT_ASSERT >= 2 */
+
+#if !defined(MPFR_GENERIC_ABI)
+
+
+
+#define uint32_t mpfr_prec_t
+#define int32_t mpfr_exp_t
+#define uint64_t mp_limb_t
+
+typedef struct MPFR_Add1sp1_state_s
+{
+  uint32_t sh;
+  int32_t bx;
+  uint64_t rb;
+  uint64_t sb;
+}
+MPFR_Add1sp1_state;
+
+static MPFR_Add1sp1_state
+MPFR_Add1sp1_mk_state(uint32_t sh, int32_t bx, uint64_t rb, uint64_t sb)
+{
+  return ((MPFR_Add1sp1_state){ .sh = sh, .bx = bx, .rb = rb, .sb = sb });
+}
+
+typedef struct K___uint64_t_int32_t_s
+{
+  uint64_t fst;
+  int32_t snd;
+}
+K___uint64_t_int32_t;
+
+typedef struct K___uint64_t_uint64_t_int32_t_s
+{
+  uint64_t fst;
+  uint64_t snd;
+  int32_t thd;
+}
+K___uint64_t_uint64_t_int32_t;
+
+#define MPFR_Lib_mpfr_struct __mpfr_struct
+#define MPFR_Exceptions_mpfr_overflow mpfr_overflow
+#define mpfr_prec _mpfr_prec
+#define mpfr_exp _mpfr_exp
+#define mpfr_d _mpfr_d
+#define mpfr_sign _mpfr_sign
+#define MPFR_Lib_gmp_NUMB_BITS GMP_NUMB_BITS
+#define MPFR_Lib_mpfr_EMAX __gmpfr_emax
+
+#define MPFR_RoundingMode_uu___is_MPFR_RNDN(rnd_mode) (rnd_mode == MPFR_RNDN)
+#define MPFR_RoundingMode_mpfr_IS_LIKE_RNDZ MPFR_IS_LIKE_RNDZ
+
+/* same as mpfr_add1sp, but for p < GMP_NUMB_BITS */
+static int
+mpfr_add1sp1 (mpfr_ptr a, mpfr_srcptr b, mpfr_srcptr c, mpfr_rnd_t rnd_mode,
+              mpfr_prec_t p)
+{
+  MPFR_Lib_mpfr_struct a0 = a[0U];
+  MPFR_Lib_mpfr_struct b0 = b[0U];
+  MPFR_Lib_mpfr_struct c0 = c[0U];
+  int32_t bx = b0.mpfr_exp;
+  int32_t cx = c0.mpfr_exp;
+  uint32_t sh = MPFR_Lib_gmp_NUMB_BITS - p;
+  MPFR_Add1sp1_state st;
+  if (bx == cx)
+  {
+    uint64_t *ap = a0.mpfr_d;
+    uint64_t *bp = b0.mpfr_d;
+    uint64_t *cp = c0.mpfr_d;
+    uint64_t a01 = (bp[0U] >> (uint32_t)1U) + (cp[0U] >> (uint32_t)1U);
+    int32_t bx1 = b0.mpfr_exp + (int32_t)1;
+    uint64_t rb = a01 & (uint64_t)1U << sh - (uint32_t)1U;
+    ap[0U] = a01 ^ rb;
+    uint64_t sb = (uint64_t)0U;
+    st = MPFR_Add1sp1_mk_state(sh, bx1, rb, sb);
+  }
+  else
+  {
+    MPFR_Add1sp1_state ite0;
+    if (bx > cx)
+    {
+      int32_t bx1 = b0.mpfr_exp;
+      int32_t cx1 = c0.mpfr_exp;
+      uint32_t d = (uint32_t)(bx1 - cx1);
+      uint64_t mask = ((uint64_t)1U << sh) - (uint64_t)1U;
+      MPFR_Add1sp1_state ite1;
+      if (d < sh)
+      {
+        uint64_t *ap = a0.mpfr_d;
+        uint64_t *bp = b0.mpfr_d;
+        uint64_t *cp = c0.mpfr_d;
+        int32_t bx2 = b0.mpfr_exp;
+        uint64_t a01 = bp[0U] + (cp[0U] >> d);
+        K___uint64_t_int32_t scrut;
+        if (a01 < bp[0U])
+          scrut =
+            (
+              (K___uint64_t_int32_t){
+                .fst = (uint64_t)0x8000000000000000U | a01 >> (uint32_t)1U,
+                .snd = bx2 + (int32_t)1
+              }
+            );
+        else
+          scrut = ((K___uint64_t_int32_t){ .fst = a01, .snd = bx2 });
+        uint64_t a02 = scrut.fst;
+        int32_t bx3 = scrut.snd;
+        uint64_t rb = a02 & (uint64_t)1U << sh - (uint32_t)1U;
+        uint64_t sb = a02 & mask ^ rb;
+        ap[0U] = a02 & ~mask;
+        ite1 = MPFR_Add1sp1_mk_state(sh, bx3, rb, sb);
+      }
+      else
+      {
+        MPFR_Add1sp1_state ite;
+        if (d < MPFR_Lib_gmp_NUMB_BITS)
+        {
+          uint64_t *ap = a0.mpfr_d;
+          uint64_t *bp = b0.mpfr_d;
+          uint64_t *cp = c0.mpfr_d;
+          int32_t bx2 = b0.mpfr_exp;
+          uint64_t sb = cp[0U] << MPFR_Lib_gmp_NUMB_BITS - d;
+          uint64_t a01 = bp[0U] + (cp[0U] >> d);
+          K___uint64_t_uint64_t_int32_t scrut;
+          if (a01 < bp[0U])
+            scrut =
+              (
+                (K___uint64_t_uint64_t_int32_t){
+                  .fst = sb | a01 & (uint64_t)1U,
+                  .snd = (uint64_t)0x8000000000000000U | a01 >> (uint32_t)1U,
+                  .thd = bx2 + (int32_t)1
+                }
+              );
+          else
+            scrut = ((K___uint64_t_uint64_t_int32_t){ .fst = sb, .snd = a01, .thd = bx2 });
+          uint64_t sb1 = scrut.fst;
+          uint64_t a02 = scrut.snd;
+          int32_t bx3 = scrut.thd;
+          uint64_t rb = a02 & (uint64_t)1U << sh - (uint32_t)1U;
+          uint64_t sb2 = sb1 | a02 & mask ^ rb;
+          ap[0U] = a02 & ~mask;
+          ite = MPFR_Add1sp1_mk_state(sh, bx3, rb, sb2);
+        }
+        else
+        {
+          uint64_t *ap = a0.mpfr_d;
+          uint64_t *bp = b0.mpfr_d;
+          int32_t bx2 = b0.mpfr_exp;
+          ap[0U] = bp[0U];
+          uint64_t rb = (uint64_t)0U;
+          uint64_t sb = (uint64_t)1U;
+          ite = MPFR_Add1sp1_mk_state(sh, bx2, rb, sb);
+        }
+        ite1 = ite;
+      }
+      ite0 = ite1;
+    }
+    else
+    {
+      int32_t bx1 = c0.mpfr_exp;
+      int32_t cx1 = b0.mpfr_exp;
+      uint32_t d = (uint32_t)(bx1 - cx1);
+      uint64_t mask = ((uint64_t)1U << sh) - (uint64_t)1U;
+      MPFR_Add1sp1_state ite1;
+      if (d < sh)
+      {
+        uint64_t *ap = a0.mpfr_d;
+        uint64_t *bp = c0.mpfr_d;
+        uint64_t *cp = b0.mpfr_d;
+        int32_t bx2 = c0.mpfr_exp;
+        uint64_t a01 = bp[0U] + (cp[0U] >> d);
+        K___uint64_t_int32_t scrut;
+        if (a01 < bp[0U])
+          scrut =
+            (
+              (K___uint64_t_int32_t){
+                .fst = (uint64_t)0x8000000000000000U | a01 >> (uint32_t)1U,
+                .snd = bx2 + (int32_t)1
+              }
+            );
+        else
+          scrut = ((K___uint64_t_int32_t){ .fst = a01, .snd = bx2 });
+        uint64_t a02 = scrut.fst;
+        int32_t bx3 = scrut.snd;
+        uint64_t rb = a02 & (uint64_t)1U << sh - (uint32_t)1U;
+        uint64_t sb = a02 & mask ^ rb;
+        ap[0U] = a02 & ~mask;
+        ite1 = MPFR_Add1sp1_mk_state(sh, bx3, rb, sb);
+      }
+      else
+      {
+        MPFR_Add1sp1_state ite;
+        if (d < MPFR_Lib_gmp_NUMB_BITS)
+        {
+          uint64_t *ap = a0.mpfr_d;
+          uint64_t *bp = c0.mpfr_d;
+          uint64_t *cp = b0.mpfr_d;
+          int32_t bx2 = c0.mpfr_exp;
+          uint64_t sb = cp[0U] << MPFR_Lib_gmp_NUMB_BITS - d;
+          uint64_t a01 = bp[0U] + (cp[0U] >> d);
+          K___uint64_t_uint64_t_int32_t scrut;
+          if (a01 < bp[0U])
+            scrut =
+              (
+                (K___uint64_t_uint64_t_int32_t){
+                  .fst = sb | a01 & (uint64_t)1U,
+                  .snd = (uint64_t)0x8000000000000000U | a01 >> (uint32_t)1U,
+                  .thd = bx2 + (int32_t)1
+                }
+              );
+          else
+            scrut = ((K___uint64_t_uint64_t_int32_t){ .fst = sb, .snd = a01, .thd = bx2 });
+          uint64_t sb1 = scrut.fst;
+          uint64_t a02 = scrut.snd;
+          int32_t bx3 = scrut.thd;
+          uint64_t rb = a02 & (uint64_t)1U << sh - (uint32_t)1U;
+          uint64_t sb2 = sb1 | a02 & mask ^ rb;
+          ap[0U] = a02 & ~mask;
+          ite = MPFR_Add1sp1_mk_state(sh, bx3, rb, sb2);
+        }
+        else
+        {
+          uint64_t *ap = a0.mpfr_d;
+          uint64_t *bp = c0.mpfr_d;
+          int32_t bx2 = c0.mpfr_exp;
+          ap[0U] = bp[0U];
+          uint64_t rb = (uint64_t)0U;
+          uint64_t sb = (uint64_t)1U;
+          ite = MPFR_Add1sp1_mk_state(sh, bx2, rb, sb);
+        }
+        ite1 = ite;
+      }
+      ite0 = ite1;
+    }
+    st = ite0;
+  }
+  if (st.bx > MPFR_Lib_mpfr_EMAX)
+  {
+    int32_t t = MPFR_Exceptions_mpfr_overflow(a, rnd_mode, a->mpfr_sign);
+    return t;
+  }
+  else
+  {
+    uint64_t *ap = a->mpfr_d;
+    uint64_t a01 = ap[0U];
+    MPFR_Lib_mpfr_struct uu___54_3461 = a[0U];
+    a[0U] =
+      (
+        (MPFR_Lib_mpfr_struct){
+          .mpfr_prec = uu___54_3461.mpfr_prec,
+          .mpfr_sign = uu___54_3461.mpfr_sign,
+          .mpfr_exp = st.bx,
+          .mpfr_d = uu___54_3461.mpfr_d
+        }
+      );
+    if (st.rb == (uint64_t)0U && st.sb == (uint64_t)0U)
+      return (int32_t)0;
+    else if (MPFR_RoundingMode_uu___is_MPFR_RNDN(rnd_mode))
+      if
+      (
+        st.rb
+        == (uint64_t)0U
+        || st.sb == (uint64_t)0U && (a01 & (uint64_t)1U << st.sh) == (uint64_t)0U
+      )
+        if (a->mpfr_sign == (int32_t)1)
+          return (int32_t)-1;
+        else
+          return (int32_t)1;
+      else
+      {
+        uint64_t *ap1 = a->mpfr_d;
+        ap1[0U] = ap1[0U] + ((uint64_t)1U << st.sh);
+        if (ap1[0U] == (uint64_t)0U)
+        {
+          ap1[0U] = (uint64_t)0x8000000000000000U;
+          if (st.bx + (int32_t)1 <= MPFR_Lib_mpfr_EMAX)
+          {
+            MPFR_Lib_mpfr_struct uu___54_3556 = a[0U];
+            a[0U] =
+              (
+                (MPFR_Lib_mpfr_struct){
+                  .mpfr_prec = uu___54_3556.mpfr_prec,
+                  .mpfr_sign = uu___54_3556.mpfr_sign,
+                  .mpfr_exp = st.bx + (int32_t)1,
+                  .mpfr_d = uu___54_3556.mpfr_d
+                }
+              );
+            return a->mpfr_sign;
+          }
+          else
+          {
+            int32_t t = MPFR_Exceptions_mpfr_overflow(a, rnd_mode, a->mpfr_sign);
+            return t;
+          }
+        }
+        else
+          return a->mpfr_sign;
+      }
+    else if (MPFR_RoundingMode_mpfr_IS_LIKE_RNDZ(rnd_mode, a->mpfr_sign < (int32_t)0))
+      if (a->mpfr_sign == (int32_t)1)
+        return (int32_t)-1;
+      else
+        return (int32_t)1;
+    else
+    {
+      uint64_t *ap1 = a->mpfr_d;
+      ap1[0U] = ap1[0U] + ((uint64_t)1U << st.sh);
+      if (ap1[0U] == (uint64_t)0U)
+      {
+        ap1[0U] = (uint64_t)0x8000000000000000U;
+        if (st.bx + (int32_t)1 <= MPFR_Lib_mpfr_EMAX)
+        {
+          MPFR_Lib_mpfr_struct uu___54_3760 = a[0U];
+          a[0U] =
+            (
+              (MPFR_Lib_mpfr_struct){
+                .mpfr_prec = uu___54_3760.mpfr_prec,
+                .mpfr_sign = uu___54_3760.mpfr_sign,
+                .mpfr_exp = st.bx + (int32_t)1,
+                .mpfr_d = uu___54_3760.mpfr_d
+              }
+            );
+          return a->mpfr_sign;
+        }
+        else
+        {
+          int32_t t = MPFR_Exceptions_mpfr_overflow(a, rnd_mode, a->mpfr_sign);
+          return t;
+        }
+      }
+      else
+        return a->mpfr_sign;
+    }
+  }
+}
+
+
+
+
+
+/* same as mpfr_add1sp, but for p = GMP_NUMB_BITS */
+static int
+mpfr_add1sp1n (mpfr_ptr a, mpfr_srcptr b, mpfr_srcptr c, mpfr_rnd_t rnd_mode)
+{
+  mpfr_exp_t bx = MPFR_GET_EXP (b);
+  mpfr_exp_t cx = MPFR_GET_EXP (c);
+  mp_limb_t *ap = MPFR_MANT(a);
+  mp_limb_t *bp = MPFR_MANT(b);
+  mp_limb_t *cp = MPFR_MANT(c);
+  mp_limb_t rb; /* round bit */
+  mp_limb_t sb; /* sticky bit */
+  mp_limb_t a0; /* to store the result */
+  mpfr_uexp_t d;
+
+  MPFR_ASSERTD(MPFR_PREC (a) == GMP_NUMB_BITS);
+  MPFR_ASSERTD(MPFR_PREC (b) == GMP_NUMB_BITS);
+  MPFR_ASSERTD(MPFR_PREC (c) == GMP_NUMB_BITS);
+
+  if (bx == cx)
+    {
+      a0 = bp[0] + cp[0];
+      rb = a0 & MPFR_LIMB_ONE;
+      ap[0] = MPFR_LIMB_HIGHBIT | (a0 >> 1);
+      bx ++;
+      sb = 0; /* since b + c fits on p+1 bits, the sticky bit is zero */
+    }
+  else if (bx > cx)
+    {
+    BGreater1:
+      d = (mpfr_uexp_t) bx - cx;
+      if (d < GMP_NUMB_BITS) /* 1 <= d < GMP_NUMB_BITS */
+        {
+          a0 = bp[0] + (cp[0] >> d);
+          sb = cp[0] << (GMP_NUMB_BITS - d); /* bits from cp[-1] after shift */
+          if (a0 < bp[0]) /* carry */
+            {
+              ap[0] = MPFR_LIMB_HIGHBIT | (a0 >> 1);
+              rb = a0 & 1;
+              bx ++;
+            }
+          else /* no carry */
+            {
+              ap[0] = a0;
+              rb = sb & MPFR_LIMB_HIGHBIT;
+              sb &= ~MPFR_LIMB_HIGHBIT;
+            }
+        }
+      else /* d >= GMP_NUMB_BITS */
+        {
+          sb = d != GMP_NUMB_BITS || cp[0] != MPFR_LIMB_HIGHBIT;
+          ap[0] = bp[0];
+          rb = d == GMP_NUMB_BITS;
+        }
+    }
+  else /* bx < cx: swap b and c */
+    {
+      mpfr_exp_t tx;
+      mp_limb_t *tp;
+      tx = bx; bx = cx; cx = tx;
+      tp = bp; bp = cp; cp = tp;
+      goto BGreater1;
+    }
+
+  /* Note: we could keep the output significand in a0 for the rounding,
+     and only store it in ap[0] at the very end, but this seems slower
+     on average (but better for the worst case). */
+
+  /* now perform rounding */
+  if (MPFR_UNLIKELY(bx > __gmpfr_emax))
+    return mpfr_overflow (a, rnd_mode, MPFR_SIGN(a));
+
+  MPFR_SET_EXP (a, bx);
+  if ((rb == 0 && sb == 0) || rnd_mode == MPFR_RNDF)
+    MPFR_RET(0);
+  else if (rnd_mode == MPFR_RNDN)
+    {
+      /* the condition below should be rb == 0 || (rb != 0 && ...), but this
+         is equivalent to rb == 0 || (...) */
+      if (rb == 0 || (sb == 0 && (ap[0] & MPFR_LIMB_ONE) == 0))
+        goto truncate;
+      else
+        goto add_one_ulp;
+    }
+  else if (MPFR_IS_LIKE_RNDZ(rnd_mode, MPFR_IS_NEG(a)))
+    {
+    truncate:
+      MPFR_RET(-MPFR_SIGN(a));
+    }
+  else /* round away from zero */
+    {
+    add_one_ulp:
+      ap[0] += MPFR_LIMB_ONE;
+      if (MPFR_UNLIKELY(ap[0] == 0))
+        {
+          ap[0] = MPFR_LIMB_HIGHBIT;
+          /* no need to have MPFR_LIKELY here, since we are in a rare branch */
+          if (bx + 1 <= __gmpfr_emax)
+            MPFR_SET_EXP (a, bx + 1);
+          else /* overflow */
+            return mpfr_overflow (a, rnd_mode, MPFR_SIGN(a));
+        }
+      MPFR_RET(MPFR_SIGN(a));
+    }
+}
+
+/* same as mpfr_add1sp, but for GMP_NUMB_BITS < p < 2*GMP_NUMB_BITS */
+static int
+mpfr_add1sp2 (mpfr_ptr a, mpfr_srcptr b, mpfr_srcptr c, mpfr_rnd_t rnd_mode,
+              mpfr_prec_t p)
+{
+  mpfr_exp_t bx = MPFR_GET_EXP (b);
+  mpfr_exp_t cx = MPFR_GET_EXP (c);
+  mp_limb_t *ap = MPFR_MANT(a);
+  mp_limb_t *bp = MPFR_MANT(b);
+  mp_limb_t *cp = MPFR_MANT(c);
+  mpfr_prec_t sh = 2*GMP_NUMB_BITS - p;
+  mp_limb_t rb; /* round bit */
+  mp_limb_t sb; /* sticky bit */
+  mp_limb_t a1, a0;
+  mp_limb_t mask;
+  mpfr_uexp_t d;
+
+  MPFR_ASSERTD(GMP_NUMB_BITS < p && p < 2 * GMP_NUMB_BITS);
+
+  if (bx == cx)
+    {
+      /* since bp[1], cp[1] >= MPFR_LIMB_HIGHBIT, a carry always occurs */
+      a0 = bp[0] + cp[0];
+      a1 = bp[1] + cp[1] + (a0 < bp[0]);
+      a0 = (a0 >> 1) | (a1 << (GMP_NUMB_BITS - 1));
+      bx ++;
+      rb = a0 & (MPFR_LIMB_ONE << (sh - 1));
+      ap[1] = MPFR_LIMB_HIGHBIT | (a1 >> 1);
+      ap[0] = a0 ^ rb;
+      sb = 0; /* since b + c fits on p+1 bits, the sticky bit is zero */
+    }
+  else if (bx > cx)
+    {
+    BGreater2:
+      d = (mpfr_uexp_t) bx - cx;
+      mask = MPFR_LIMB_MASK(sh);
+      if (d < GMP_NUMB_BITS) /* 0 < d < GMP_NUMB_BITS */
+        {
+          sb = cp[0] << (GMP_NUMB_BITS - d); /* bits from cp[-1] after shift */
+          a0 = bp[0] + ((cp[1] << (GMP_NUMB_BITS - d)) | (cp[0] >> d));
+          a1 = bp[1] + (cp[1] >> d) + (a0 < bp[0]);
+          if (a1 < bp[1]) /* carry in high word */
+            {
+            exponent_shift:
+              sb |= a0 & 1;
+              /* shift a by 1 */
+              a0 = (a1 << (GMP_NUMB_BITS - 1)) | (a0 >> 1);
+              ap[1] = MPFR_LIMB_HIGHBIT | (a1 >> 1);
+              bx ++;
+            }
+          else
+            ap[1] = a1;
+          rb = a0 & (MPFR_LIMB_ONE << (sh - 1));
+          sb |= (a0 & mask) ^ rb;
+          ap[0] = a0 & ~mask;
+        }
+      else if (d < 2*GMP_NUMB_BITS) /* GMP_NUMB_BITS <= d < 2*GMP_NUMB_BITS */
+        {
+          sb = (d == GMP_NUMB_BITS) ? cp[0]
+            : cp[0] | (cp[1] << (2*GMP_NUMB_BITS-d));
+          a0 = bp[0] + (cp[1] >> (d - GMP_NUMB_BITS));
+          a1 = bp[1] + (a0 < bp[0]);
+          if (a1 == 0)
+            goto exponent_shift;
+          rb = a0 & (MPFR_LIMB_ONE << (sh - 1));
+          sb |= (a0 & mask) ^ rb;
+          ap[0] = a0 & ~mask;
+          ap[1] = a1;
+        }
+      else /* d >= 2*GMP_NUMB_BITS */
+        {
+          ap[0] = bp[0];
+          ap[1] = bp[1];
+          rb = 0; /* since p < 2*GMP_NUMB_BITS */
+          sb = 1; /* since c <> 0 */
+        }
+    }
+  else /* bx < cx: swap b and c */
+    {
+      mpfr_exp_t tx;
+      mp_limb_t *tp;
+      tx = bx; bx = cx; cx = tx;
+      tp = bp; bp = cp; cp = tp;
+      goto BGreater2;
+    }
+
+  /* now perform rounding */
+  if (MPFR_UNLIKELY(bx > __gmpfr_emax))
+    return mpfr_overflow (a, rnd_mode, MPFR_SIGN(a));
+
+  MPFR_SET_EXP (a, bx);
+  if ((rb == 0 && sb == 0) || rnd_mode == MPFR_RNDF)
+    MPFR_RET(0);
+  else if (rnd_mode == MPFR_RNDN)
+    {
+      if (rb == 0 || (sb == 0 && (ap[0] & (MPFR_LIMB_ONE << sh)) == 0))
+        goto truncate;
+      else
+        goto add_one_ulp;
+    }
+  else if (MPFR_IS_LIKE_RNDZ(rnd_mode, MPFR_IS_NEG(a)))
+    {
+    truncate:
+      MPFR_RET(-MPFR_SIGN(a));
+    }
+  else /* round away from zero */
+    {
+    add_one_ulp:
+      ap[0] += MPFR_LIMB_ONE << sh;
+      ap[1] += (ap[0] == 0);
+      if (MPFR_UNLIKELY(ap[1] == 0))
+        {
+          ap[1] = MPFR_LIMB_HIGHBIT;
+          /* no need to have MPFR_LIKELY here, since we are in a rare branch */
+          if (bx + 1 <= __gmpfr_emax)
+            MPFR_SET_EXP (a, bx + 1);
+          else /* overflow */
+            return mpfr_overflow (a, rnd_mode, MPFR_SIGN(a));
+        }
+      MPFR_RET(MPFR_SIGN(a));
+    }
+}
+
+/* same as mpfr_add1sp, but for 2*GMP_NUMB_BITS < p < 3*GMP_NUMB_BITS */
+static int
+mpfr_add1sp3 (mpfr_ptr a, mpfr_srcptr b, mpfr_srcptr c, mpfr_rnd_t rnd_mode,
+              mpfr_prec_t p)
+{
+  mpfr_exp_t bx = MPFR_GET_EXP (b);
+  mpfr_exp_t cx = MPFR_GET_EXP (c);
+  mp_limb_t *ap = MPFR_MANT(a);
+  mp_limb_t *bp = MPFR_MANT(b);
+  mp_limb_t *cp = MPFR_MANT(c);
+  mpfr_prec_t sh = 3*GMP_NUMB_BITS - p;
+  mp_limb_t rb; /* round bit */
+  mp_limb_t sb; /* sticky bit */
+  mp_limb_t a2, a1, a0;
+  mp_limb_t mask;
+  mpfr_uexp_t d;
+
+  MPFR_ASSERTD(2 * GMP_NUMB_BITS < p && p < 3 * GMP_NUMB_BITS);
+
+  if (bx == cx)
+    {
+      /* since bp[2], cp[2] >= MPFR_LIMB_HIGHBIT, a carry always occurs */
+      a0 = bp[0] + cp[0];
+      a1 = bp[1] + cp[1] + (a0 < bp[0]);
+      a2 = bp[2] + cp[2] + (a1 < bp[1] || (a1 == bp[1] && a0 < bp[0]));
+      /* since p < 3 * GMP_NUMB_BITS, we lose no bit in a0 >> 1 */
+      a0 = (a1 << (GMP_NUMB_BITS - 1)) | (a0 >> 1);
+      bx ++;
+      rb = a0 & (MPFR_LIMB_ONE << (sh - 1));
+      ap[2] = MPFR_LIMB_HIGHBIT | (a2 >> 1);
+      ap[1] = (a2 << (GMP_NUMB_BITS - 1)) | (a1 >> 1);
+      ap[0] = a0 ^ rb;
+      sb = 0; /* since b + c fits on p+1 bits, the sticky bit is zero */
+    }
+  else if (bx > cx)
+    {
+    BGreater2:
+      d = (mpfr_uexp_t) bx - cx;
+      mask = MPFR_LIMB_MASK(sh);
+      if (d < GMP_NUMB_BITS) /* 0 < d < GMP_NUMB_BITS */
+        {
+          mp_limb_t cy;
+          sb = cp[0] << (GMP_NUMB_BITS - d); /* bits from cp[-1] after shift */
+          a0 = bp[0] + ((cp[1] << (GMP_NUMB_BITS - d)) | (cp[0] >> d));
+          a1 = bp[1] + ((cp[2] << (GMP_NUMB_BITS - d)) | (cp[1] >> d))
+            + (a0 < bp[0]);
+          cy = a1 < bp[1] || (a1 == bp[1] && a0 < bp[0]); /* carry in a1 */
+          a2 = bp[2] + (cp[2] >> d) + cy;
+          if (a2 < bp[2] || (a2 == bp[2] && cy)) /* carry in high word */
+            {
+            exponent_shift:
+              sb |= a0 & 1;
+              /* shift a by 1 */
+              a0 = (a1 << (GMP_NUMB_BITS - 1)) | (a0 >> 1);
+              ap[1] = (a2 << (GMP_NUMB_BITS - 1)) | (a1 >> 1);
+              ap[2] = MPFR_LIMB_HIGHBIT | (a2 >> 1);
+              bx ++;
+            }
+          else
+            {
+              ap[1] = a1;
+              ap[2] = a2;
+            }
+          rb = a0 & (MPFR_LIMB_ONE << (sh - 1));
+          sb |= (a0 & mask) ^ rb;
+          ap[0] = a0 & ~mask;
+        }
+      else if (d < 2*GMP_NUMB_BITS) /* GMP_NUMB_BITS <= d < 2*GMP_NUMB_BITS */
+        {
+          mp_limb_t c0shifted;
+          sb = (d == GMP_NUMB_BITS) ? cp[0]
+            : (cp[1] << (2*GMP_NUMB_BITS - d)) | cp[0];
+          c0shifted = (d == GMP_NUMB_BITS) ? cp[1]
+            : (cp[2] << (2*GMP_NUMB_BITS-d)) | (cp[1] >> (d - GMP_NUMB_BITS));
+          a0 = bp[0] + c0shifted;
+          a1 = bp[1] + (cp[2] >> (d - GMP_NUMB_BITS)) + (a0 < bp[0]);
+          /* if a1 < bp[1], there was a carry in the above addition,
+             or when a1 = bp[1] and one of the added terms is nonzero
+             (the sum of cp[2] >> (d - GMP_NUMB_BITS) and a0 < bp[0]
+             is at most 2^GMP_NUMB_BITS-d) */
+          a2 = bp[2] + ((a1 < bp[1]) || (a1 == bp[1] && a0 < bp[0]));
+          if (a2 == 0)
+            goto exponent_shift;
+          rb = a0 & (MPFR_LIMB_ONE << (sh - 1));
+          sb |= (a0 & mask) ^ rb;
+          ap[0] = a0 & ~mask;
+          ap[1] = a1;
+          ap[2] = a2;
+        }
+      else if (d < 3*GMP_NUMB_BITS) /* 2*GMP_NUMB_BITS<=d<3*GMP_NUMB_BITS */
+        {
+          MPFR_ASSERTD (2*GMP_NUMB_BITS <= d && d < 3*GMP_NUMB_BITS);
+          sb = (d == 2*GMP_NUMB_BITS ? 0 : cp[2] << (3*GMP_NUMB_BITS - d))
+            | cp[1] | cp[0];
+          a0 = bp[0] + (cp[2] >> (d - 2*GMP_NUMB_BITS));
+          a1 = bp[1] + (a0 < bp[0]);
+          a2 = bp[2] + (a1 < bp[1]);
+          if (a2 == 0)
+            goto exponent_shift;
+          rb = a0 & (MPFR_LIMB_ONE << (sh - 1));
+          sb |= (a0 & mask) ^ rb;
+          ap[0] = a0 & ~mask;
+          ap[1] = a1;
+          ap[2] = a2;
+        }
+      else /* d >= 2*GMP_NUMB_BITS */
+        {
+          ap[0] = bp[0];
+          ap[1] = bp[1];
+          ap[2] = bp[2];
+          rb = 0; /* since p < 3*GMP_NUMB_BITS */
+          sb = 1; /* since c <> 0 */
+        }
+    }
+  else /* bx < cx: swap b and c */
+    {
+      mpfr_exp_t tx;
+      mp_limb_t *tp;
+      tx = bx; bx = cx; cx = tx;
+      tp = bp; bp = cp; cp = tp;
+      goto BGreater2;
+    }
+
+  /* now perform rounding */
+  if (MPFR_UNLIKELY(bx > __gmpfr_emax))
+    return mpfr_overflow (a, rnd_mode, MPFR_SIGN(a));
+
+  MPFR_SET_EXP (a, bx);
+  if ((rb == 0 && sb == 0) || rnd_mode == MPFR_RNDF)
+    MPFR_RET(0);
+  else if (rnd_mode == MPFR_RNDN)
+    {
+      if (rb == 0 || (sb == 0 && (ap[0] & (MPFR_LIMB_ONE << sh)) == 0))
+        goto truncate;
+      else
+        goto add_one_ulp;
+    }
+  else if (MPFR_IS_LIKE_RNDZ(rnd_mode, MPFR_IS_NEG(a)))
+    {
+    truncate:
+      MPFR_RET(-MPFR_SIGN(a));
+    }
+  else /* round away from zero */
+    {
+    add_one_ulp:
+      ap[0] += MPFR_LIMB_ONE << sh;
+      ap[1] += (ap[0] == 0);
+      ap[2] += (ap[1] == 0 && ap[0] == 0);
+      if (MPFR_UNLIKELY(ap[2] == 0))
+        {
+          ap[2] = MPFR_LIMB_HIGHBIT;
+          /* no need to have MPFR_LIKELY here, since we are in a rare branch */
+          if (bx + 1 <= __gmpfr_emax)
+            MPFR_SET_EXP (a, bx + 1);
+          else /* overflow */
+            return mpfr_overflow (a, rnd_mode, MPFR_SIGN(a));
+        }
+      MPFR_RET(MPFR_SIGN(a));
+    }
+}
+
+#endif /* !defined(MPFR_GENERIC_ABI) */
+
+/* {ap, n} <- {bp, n} + {cp + q, n - q} >> r where d = q * GMP_NUMB_BITS + r.
+   Return the carry at ap[n+1] (0 or 1) and set *low so that:
+   * the most significant bit of *low would be that of ap[-1] if we would
+     compute one more limb of the (infinite) addition
+   * the GMP_NUMB_BITS-1 least significant bits of *low are zero iff all bits
+     of ap[-1], ap[-2], ... would be zero (except the most significant bit
+     of ap[-1).
+   Assume 0 < d < GMP_NUMB_BITS*n. */
+static mp_limb_t
+mpfr_addrsh (mp_limb_t *ap, mp_limb_t *bp, mp_limb_t *cp, mp_size_t n,
+             mp_size_t d, mp_limb_t *low)
+{
+  mp_limb_t cy, cy2, c_shifted;
+  mp_size_t i;
+
+  if (d < GMP_NUMB_BITS)
+    {
+      /* {ap, n} <- {bp, n} + {cp, n} >> d */
+      MPFR_ASSERTD (d > 0);
+      /* thus 0 < GMP_NUMB_BITS - d < GMP_NUMB_BITS */
+      *low = cp[0] << (GMP_NUMB_BITS - d);
+      for (i = 0, cy = 0; i < n - 1; i++)
+        {
+          c_shifted = (cp[i+1] << (GMP_NUMB_BITS - d)) | (cp[i] >> d);
+          ap[i] = bp[i] + c_shifted;
+          cy2 = ap[i] < c_shifted;
+          ap[i] += cy;
+          cy = cy2 + (ap[i] < cy);
+        }
+      /* most significant limb is special */
+      c_shifted = cp[i] >> d;
+      ap[i] = bp[i] + c_shifted;
+      cy2 = ap[i] < c_shifted;
+      ap[i] += cy;
+      cy = cy2 + (ap[i] < cy);
+    }
+  else /* d >= GMP_NUMB_BITS */
+    {
+      mp_size_t q = d / GMP_NUMB_BITS;
+      mpfr_uexp_t r = d % GMP_NUMB_BITS;
+      if (r == 0)
+        {
+          MPFR_ASSERTD(q > 0);
+          *low = cp[q-1];
+          for (i = 0; i < q-1; i++)
+            *low |= !!cp[i];
+          cy = mpn_add_n (ap, bp, cp + q, n - q);
+          cy = mpn_add_1 (ap + n - q, bp + n - q, q, cy);
+        }
+      else /* 0 < r < GMP_NUMB_BITS */
+        {
+          *low = cp[q] << (GMP_NUMB_BITS - r);
+          for (i = 0; i < q; i++)
+            *low |= !!cp[i];
+          for (i = 0, cy = 0; i < n - q - 1; i++)
+            {
+              c_shifted = (cp[q+i+1] << (GMP_NUMB_BITS - r)) | (cp[q+i] >> r);
+              ap[i] = bp[i] + c_shifted;
+              cy2 = ap[i] < c_shifted;
+              ap[i] += cy;
+              cy = cy2 + (ap[i] < cy);
+            }
+          /* most significant limb of c is special */
+          MPFR_ASSERTD(i == n - q - 1);
+          c_shifted = cp[n-1] >> r;
+          ap[i] = bp[i] + c_shifted;
+          cy2 = ap[i] < c_shifted;
+          ap[i] += cy;
+          cy = cy2 + (ap[i] < cy);
+          /* upper limbs are copied */
+          cy = mpn_add_1 (ap + n - q, bp + n - q, q, cy);
+        }
+    }
+  return cy;
+}
+
+/* compute sign(b) * (|b| + |c|).
+   Returns 0 iff result is exact,
+   a negative value when the result is less than the exact value,
+   a positive value otherwise. */
+MPFR_HOT_FUNCTION_ATTR int
+mpfr_add1sp (mpfr_ptr a, mpfr_srcptr b, mpfr_srcptr c, mpfr_rnd_t rnd_mode)
+{
+  mpfr_uexp_t d;
+  mpfr_prec_t p;
+  unsigned int sh;
+  mp_size_t n;
+  mp_limb_t *ap = MPFR_MANT(a);
+  mpfr_exp_t bx;
+  mp_limb_t limb, rb, sb;
+  int inexact;
+  int neg;
+
+  MPFR_ASSERTD(MPFR_PREC(a) == MPFR_PREC(b) && MPFR_PREC(b) == MPFR_PREC(c));
+  MPFR_ASSERTD(MPFR_IS_PURE_FP(b));
+  MPFR_ASSERTD(MPFR_IS_PURE_FP(c));
+
+  MPFR_SET_SAME_SIGN (a, b);
+
+  /* Read prec and num of limbs */
+  p = MPFR_GET_PREC (b);
+
+#if !defined(MPFR_GENERIC_ABI)
+  if (p < GMP_NUMB_BITS)
+    return mpfr_add1sp1 (a, b, c, rnd_mode, p);
+
+  if (GMP_NUMB_BITS < p && p < 2 * GMP_NUMB_BITS)
+    return mpfr_add1sp2 (a, b, c, rnd_mode, p);
+
+  /* we put this test after the mpfr_add1sp2() call, to avoid slowing down
+     the more frequent case GMP_NUMB_BITS < p < 2 * GMP_NUMB_BITS */
+  if (p == GMP_NUMB_BITS)
+    return mpfr_add1sp1n (a, b, c, rnd_mode);
+
+  if (2 * GMP_NUMB_BITS < p && p < 3 * GMP_NUMB_BITS)
+    return mpfr_add1sp3 (a, b, c, rnd_mode, p);
+#endif
+
+  /* We need to get the sign before the possible exchange. */
+  neg = MPFR_IS_NEG (b);
+
+  bx = MPFR_GET_EXP(b);
+  if (bx < MPFR_GET_EXP(c))
+    {
+      mpfr_srcptr t = b;
+      bx = MPFR_GET_EXP(c);
+      b = c;
+      c = t;
+    }
+  MPFR_ASSERTD(bx >= MPFR_GET_EXP(c));
+
+  n = MPFR_PREC2LIMBS (p);
+  MPFR_UNSIGNED_MINUS_MODULO(sh, p);
+  d = (mpfr_uexp_t) (bx - MPFR_GET_EXP(c));
+
+  /* printf ("New add1sp with diff=%lu\n", (unsigned long) d); */
+
+  if (d == 0)
+    {
+      /* d==0 */
+      /* mpfr_print_mant_binary("C= ", MPFR_MANT(c), p); */
+      /* mpfr_print_mant_binary("B= ", MPFR_MANT(b), p); */
+      bx++;                                /* exp + 1 */
+      limb = mpn_add_n (ap, MPFR_MANT(b), MPFR_MANT(c), n);
+      /* mpfr_print_mant_binary("A= ", ap, p); */
+      MPFR_ASSERTD(limb != 0);             /* There must be a carry */
+      rb = ap[0] & (MPFR_LIMB_ONE << sh);  /* Get round bit (sb=0) */
+      mpn_rshift (ap, ap, n, 1);           /* Shift mantissa A */
+      ap[n-1] |= MPFR_LIMB_HIGHBIT;        /* Set MSB */
+      ap[0]   &= ~MPFR_LIMB_MASK(sh);      /* Clear round bit */
+
+
+      /* Fast track for faithful rounding: since b and c have the same
+         precision and the same exponent, the neglected value is either
+         0 or 1/2 ulp(a), thus returning a is fine. */
+      if (rnd_mode == MPFR_RNDF)
+        { inexact = 0; goto set_exponent; }
+
+      if (rb == 0) /* Check exact case */
+        { inexact = 0; goto set_exponent; }
+
+      /* Zero: Truncate
+         Nearest: Even Rule => truncate or add 1
+         Away: Add 1 */
+      if (MPFR_LIKELY (rnd_mode == MPFR_RNDN))
+        {
+          if ((ap[0] & (MPFR_LIMB_ONE << sh)) == 0)
+            { inexact = -1; goto set_exponent; }
+          else
+            goto add_one_ulp;
+        }
+      MPFR_UPDATE_RND_MODE(rnd_mode, neg);
+      if (rnd_mode == MPFR_RNDZ)
+        { inexact = -1; goto set_exponent; }
+      else
+        goto add_one_ulp;
+    }
+  else if (MPFR_UNLIKELY (d >= p))
+    {
+      /* fast track for RNDF */
+      if (MPFR_LIKELY(rnd_mode == MPFR_RNDF))
+        goto copy_set_exponent;
+
+      if (MPFR_LIKELY (d > p))
+        {
+          /* d > p : Copy B in A */
+          /* Away:    Add 1
+             Nearest: Trunc
+             Zero:    Trunc */
+          if (rnd_mode == MPFR_RNDN || MPFR_IS_LIKE_RNDZ (rnd_mode, neg))
+            {
+            copy_set_exponent:
+              if (a != b)
+                MPN_COPY (ap, MPFR_MANT(b), n);
+              inexact = -1;
+              goto set_exponent;
+            }
+          else
+            {
+            copy_add_one_ulp:
+              if (a != b)
+                MPN_COPY (ap, MPFR_MANT(b), n);
+              goto add_one_ulp;
+            }
+        }
+      else
+        {
+          /* d==p : Copy B in A */
+          /* Away:     Add 1
+             Nearest:  Even Rule if C is a power of 2, else Add 1
+             Zero:     Trunc */
+          if (rnd_mode == MPFR_RNDN)
+            {
+              /* Check if C was a power of 2 */
+              if (mpfr_powerof2_raw (c) &&
+                  ((MPFR_MANT (b))[0] & (MPFR_LIMB_ONE << sh)) == 0)
+                goto copy_set_exponent;
+              /* Not a Power of 2 */
+              goto copy_add_one_ulp;
+            }
+          else if (MPFR_IS_LIKE_RNDZ (rnd_mode, neg))
+            goto copy_set_exponent;
+          else
+            goto copy_add_one_ulp;
+        }
+    }
+  else /* 0 < d < p */
+    {
+      mp_limb_t mask = ~MPFR_LIMB_MASK(sh);
+
+      /* General case: 1 <= d < p */
+
+      limb = mpfr_addrsh (ap, MPFR_MANT(b), MPFR_MANT(c), n, d, &sb);
+      /* the most significant bit of sb contains what would be the most
+         significant bit of ap[-1], and the remaining bits of sb are 0
+         iff the remaining bits of ap[-1], ap[-2], ... are all zero */
+
+      if (sh > 0)
+        {
+          /* The round bit and a part of the sticky bit are in ap[0]. */
+          rb = (ap[0] & (MPFR_LIMB_ONE << (sh - 1)));
+          sb |= ap[0] & MPFR_LIMB_MASK (sh - 1);
+        }
+      else
+        {
+          /* The round bit and possibly a part of the sticky bit are
+             in sb. */
+          rb = sb & MPFR_LIMB_HIGHBIT;
+          sb &= ~MPFR_LIMB_HIGHBIT;
+        }
+
+      ap[0] &= mask;
+
+      /* Check for carry out */
+      if (MPFR_UNLIKELY (limb != 0))
+        {
+          limb = ap[0] & (MPFR_LIMB_ONE << sh); /* Get LSB (will be new rb) */
+          mpn_rshift (ap, ap, n, 1);            /* Shift significand */
+          bx++;                                 /* Increase exponent */
+          ap[n-1] |= MPFR_LIMB_HIGHBIT;         /* Set MSB */
+          ap[0]   &= mask;                      /* Clear LSB */
+          sb      |= rb;                        /* Update sb */
+          rb      = limb;                       /* New rb */
+          /* printf ("(Overflow) rb=%lu sb=%lu\n",
+             (unsigned long) rb, (unsigned long) sb);
+             mpfr_print_mant_binary ("Add=  ", ap, p); */
+        }
+
+      /* Round:
+          Zero: Truncate but could be exact.
+          Away: Add 1 if rb or sb !=0
+          Nearest: Truncate but could be exact if sb==0
+                   Add 1 if rb !=0,
+                   Even rule else */
+      if (MPFR_LIKELY(rnd_mode == MPFR_RNDF))
+        { inexact = 0; goto set_exponent; }
+      else if (rnd_mode == MPFR_RNDN)
+        {
+          inexact = - (sb != 0);
+          if (rb == 0)
+            goto set_exponent;
+          else if (MPFR_UNLIKELY (sb == 0) &&
+                   (ap[0] & (MPFR_LIMB_ONE << sh)) == 0)
+            { inexact = -1; goto set_exponent; }
+          else
+            goto add_one_ulp;
+        }
+      MPFR_UPDATE_RND_MODE(rnd_mode, neg);
+      inexact = - (rb != 0 || sb != 0);
+      if (rnd_mode == MPFR_RNDZ || inexact == 0)
+        goto set_exponent;
+      else
+        goto add_one_ulp;
+    }
+  MPFR_RET_NEVER_GO_HERE();
+
+ add_one_ulp:
+  /* add one unit in last place to a */
+  /* printf("AddOneUlp\n"); */
+  if (MPFR_UNLIKELY (mpn_add_1 (ap, ap, n, MPFR_LIMB_ONE << sh)))
+    {
+      /* Case 100000x0 = 0x1111x1 + 1*/
+      /* printf("Pow of 2\n"); */
+      bx++;
+      ap[n-1] = MPFR_LIMB_HIGHBIT;
+    }
+  inexact = 1;
+
+ set_exponent:
+  if (MPFR_UNLIKELY(bx > __gmpfr_emax)) /* Check for overflow */
+    {
+      /* printf("Overflow\n"); */
+      return mpfr_overflow (a, rnd_mode, MPFR_SIGN(a));
+    }
+  MPFR_SET_EXP (a, bx);
+
+  MPFR_RET (inexact * MPFR_INT_SIGN (a));
+}
