code/mpfr/MPFR.fst
@@ -1,3 +1,4 @@
 module MPFR
 
 let mpfr_add1sp1 = MPFR.Add1sp1.mpfr_add1sp1
+let mpfr_mul_1 = MPFR.Mul_1.mpfr_mul_1
